## Résolution générale par la méthode de Cramer (n = 2)


```math
%34o$$%34c
||{"id":166722548948}||
ax + by = c
ax + by = c'

<=>
a'ax + a'by = a'c
-a'ax - ab^y = -c'a

<=>
a'ax + a'by = a'c
(1 + 2)
(a'b-a'b)y = a'c - ac'

<=>
\{a'ax + a'by = a'c
 y = {a'c- ac'}/{a'b-ab'}
%34o$$%34c
\}


<=>
ab'x + bb'y = b'c
-a'bx - bb'y = -bc'

<=>(1+2)
(ab'-a'b)x = b'c - bc'
-a'bx - bb'y = -bc'

<=> 
x = {b'c - bc'}/{ab'-a'b}
-a'bx - bb'y = -bc'

S = \{({b'c -bc'}/{ab'-a'b}; {a'c - ac'}/{a'b-ab'})\} * 1 = {-1}/{-1}


= \{({b'c -bc'}/{ab'-a'b}; {a'c - ac'}/{ab'-a'b})\}

```
